lib_misc/SteelPtrdiff.fst
@@ -13,53 +13,63 @@ open Utils2
 // add hypothesis about whether the returned value actually fits on ptrdiff_t
 // that is, explicit the fact that the implemented allocator relies on the ">= 32-bit" assumption
 // TODO: convert back to UP
-assume val ptrdiff (#a: Type) (ptr1 ptr2: A.ptr a)
+assume val ptrdiff' (#a: Type) (arr1 arr2: array a)
   : Pure UP.t
-  (requires A.base ptr1 == A.base ptr2)
+  (requires same_base_array arr1 arr2)
   (ensures fun r ->
-    UP.v r == A.offset ptr1 - A.offset ptr2
+    UP.v r == A.offset (A.ptr_of arr1) - A.offset (A.ptr_of arr2)
   )
 
-assume val u32_to_z (x: U32.t)
-  : Pure UP.t
-  (requires US.fits_u32 /\ U32.v x < pow2 31)
-  (ensures fun r -> UP.v r == U32.v x)
 
+
+assume val ptrdiff (#a: Type) (arr1 arr2: array a)
+  : Steel UP.t
+  (A.varray arr1 `star` A.varray arr2)
+  (fun _ -> A.varray arr1 `star` A.varray arr2)
+  (requires fun _ -> same_base_array arr1 arr2)
+  (ensures fun h0 r h1 ->
+    A.asel arr1 h1 == A.asel arr1 h0 /\
+    A.asel arr2 h1 == A.asel arr2 h0 /\
+    UP.v r == A.offset (A.ptr_of arr1) - A.offset (A.ptr_of arr2)
+  )
+
+//assume val u32_to_z (x: U32.t)
+//  : Pure UP.t
+//  (requires US.fits_u32 /\ U32.v x < pow2 31)
+//  (ensures fun r -> UP.v r == U32.v x)
+
+// OK
 assume val sz_to_u32 (x: US.t)
   : Pure U32.t
   (requires US.fits_u32)
   (ensures fun r -> U32.v r = US.v x)
 
-assume val z_to_u32 (x: UP.t)
-  : Pure U32.t
-  (requires US.fits_u32 /\ UP.v x >= 0)
-  (ensures fun r -> U32.v r = UP.v x)
-
+// OK
 assume val z_to_sz (x: UP.t)
   : Pure US.t
   (requires UP.v x >= 0)
   (ensures fun r -> US.v r = UP.v x)
 
-assume val fits_lte (x y: nat) : Lemma
-  (requires (x <= y /\ UP.fits y))
-  (ensures (UP.fits x))
-  [SMTPat (UP.fits x); SMTPat (UP.fits y)]
+//assume val fits_lte (x y: nat) : Lemma
+//  (requires (x <= y /\ UP.fits y))
+//  (ensures (UP.fits x))
+//  [SMTPat (UP.fits x); SMTPat (UP.fits y)]
 
-let mod_spec (a:nat{UP.fits a}) (b:nat{UP.fits b /\ b <> 0}) : GTot (n:nat{UP.fits n}) =
-  let open FStar.Mul in
-  let res = a - ((a/b) * b) in
-  fits_lte res a;
-  res
-
-// TODO: check why SizeT uses mod_spec
-assume val rem (a: UP.t) (b: UP.t{UP.v b > 0}) : Pure UP.t
-  (requires True)
-  (ensures (fun c -> admit (); mod_spec (UP.v a) (UP.v b) == UP.v c))
-
-
-assume val div (a: UP.t) (b: UP.t{UP.v b > 0}) : Pure UP.t
-  (requires True)
-  (ensures (fun c -> (UP.v a) / (UP.v b) == UP.v c))
+//let mod_spec (a:nat{UP.fits a}) (b:nat{UP.fits b /\ b <> 0}) : GTot (n:nat{UP.fits n}) =
+//  let open FStar.Mul in
+//  let res = a - ((a/b) * b) in
+//  fits_lte res a;
+//  res
+//
+//// TODO: check why SizeT uses mod_spec
+//assume val rem (a: UP.t) (b: UP.t{UP.v b > 0}) : Pure UP.t
+//  (requires True)
+//  (ensures (fun c -> admit (); mod_spec (UP.v a) (UP.v b) == UP.v c))
+//
+//
+//assume val div (a: UP.t) (b: UP.t{UP.v b > 0}) : Pure UP.t
+//  (requires True)
+//  (ensures (fun c -> (UP.v a) / (UP.v b) == UP.v c))
 
 
 // uintptr_t modelization
